# 一阶线性常系数递归表达式

## 形式

形如
$$
a_{n}=c_{1} a_{n-1}+c_{2} a_{n-2}+\cdots+c_{k} a_{n-k}
$$
where $c_{1}, c_{2}, \cdots, c_{k}$ are real number, and $c_{k} \neq 0$

## 解法

### degree = 2

$$
a_{n}=c_{1} a_{n-1}+c_{2} a_{n-2}
$$

考虑方程
$$
r^2-c_1r-c_2 = 0
$$
两个根$r_1,r_2$

* 如果$r_1 \not= r_2$
  则获得解的形式为

$$
a_n = \alpha _1 r_1^n + \alpha _2 r_2 ^n
$$

​		代入初始条件就可以得到解

* 如果重根

  则获得解的形式为
  $$
  a_n = \alpha _1 r^n + \alpha _2 nr ^n
  $$
  代入初始条件就可以得到解

### degree $\ge$2的一般情况

Theorem Let $c_{1}, \cdots, c_{k}$ be real numbers. Suppose that the characteristic equation $r^{k}-c_{1} r^{k-1}-\cdots-c_{k}=0$ has $t$ distinct roots $r_{1}, \cdots, r_{t}$ with multiplicities $m_{1}, \cdots, m_{t},$ respectively, so that $m_{i} \geq 1$ for $i=1,2, \cdots, t$ and $m_{1}+m_{2}+$ $\cdots+m_{t}=k .$ Then the sequence $\left\{a_{n}\right\}$ is a solution of the recurrence relation $a_{n}=c_{1} a_{n-1}+c_{2} a_{n-2}+\cdots+c_{k} a_{n-k}$ iff
$$
\begin{aligned}
a_{n} &=\left(\alpha_{1,0}+\alpha_{1,1} n+\cdots+\alpha_{1, m_{1}} n^{m_{1}-1}\right) r_{1}^{n} \\
&+\left(\alpha_{2,0}+\alpha_{2,1} n+\cdots+\alpha_{2, m_{2}} n^{m_{2}-1}\right) r_{2}^{n} \\
&+\cdots+\left(\alpha_{t, 0}+\alpha_{t, 1} n+\cdots+\alpha_{t, m_{t}} n^{m_{t}-1}\right) r_{t}^{n}
\end{aligned}
$$
for $n=0,1,2, \cdots,$ where $\alpha_{i, j}$ are constants.



## 一节线性常系数非齐次递归表达式的求解

Theorem: Suppose that $\left\{a_{n}\right\}$ satisfies the linear non-homogeneous recurrence relation

 $a_{n}=c_{1} a_{n-1}+c_{2} a_{n-2}+$ $\cdots+c_{k} a_{n-k}+F(n)$ 

where $c_{1}, \cdots, c_{k}$ are real numbers, and $F(n)=\left(b_{t} n^{t}+b_{t-1} n^{t-1}+\cdots+b_{1} n+b_{0}\right) s^{n},$ where $b_{1}, \cdots, b_{t}$and $s$ are real numbers.
1) When $s$ is not a characteristic root of the associated linear homogeneous recurrence relation, there is a particular solution of the form
$$
\left(p_{t} n^{t}+p_{t-1} n^{t-1}+\cdots+p_{1} n+p_{0}\right) s^{n}
$$
2) When $s$ is a characteristic root with multiplicity $m$, there is a particular solution of the form
$$
n^{m}\left(p_{t} n^{t}+p_{t-1} n^{t-1}+\cdots+p_{1} n+p_{0}\right) s^{n}
$$